combine files

LeanScratch/Untyped/Shifting.lean
@@ -1,5 +1,58 @@
 import LeanScratch.Untyped.Basic
 
+-- Pierce definition 6.1.2
+inductive Term.free : Term → ℕ → Prop where
+| var {k n: ℕ} : k < n → free (var k) n
+| abs {n' : ℕ} {t₁ : Term} : free t₁ (n'+1) → free (abs t₁) n'
+| app {n : ℕ} {t₁ t₂ : Term} : free t₁ n → free t₂ n → free (app t₁ t₂) n
+
+-- Pierce exercise 6.2.6
+theorem Term.free_shiftₙ (t : Term) (n c d: ℕ) (h : free t n) : free (t.shiftₙ c d) (n+d) := by
+  revert c
+  revert n
+  induction t <;> intros n h c <;> simp [shiftₙ]
+
+  case var x =>
+    cases h with | var h => 
+    by_cases h' : x < c <;> simp [h'] <;> apply free.var 
+    · exact Nat.lt_add_right d h
+    · exact Nat.add_lt_add_right h d 
+
+  case app l r l_ih r_ih =>
+    cases h with | app hl hr =>
+    apply free.app
+    · exact l_ih n hl c
+    · exact r_ih n hr c
+
+  case abs body ih =>
+    apply free.abs
+    induction body <;> rw [←Nat.add_right_comm n 1 d]
+    case a.var x' =>
+      simp [shiftₙ]
+      by_cases h' : x' < c + 1 
+      <;> simp [h'] 
+      <;> apply free.var
+      <;> cases h
+      <;> rename_i h
+      <;> cases ih (n+1) h (c+1)
+      <;> rename_i h''
+      <;> simp [h'] at h''
+      · exact h''
+      · exact Nat.add_lt_add_right h'' d
+    case a.abs body ih' =>
+       apply free.abs
+       cases h with | abs h' =>
+       cases ih (n+1) h' (c+1) with | abs h'' =>
+       exact h''
+    case a.app l' r' lih' rih' =>
+       apply free.app
+       <;> cases h
+       <;> rename_i h
+       <;> cases ih (n+1) h (c+1)
+       <;> rename_i l r
+       · exact l
+       · exact r
+
 -- much thanks to https://github.com/pi8027/lambda-calculus/blob/master/agda/Lambda/Confluence.agda
 
 -- TODO: these all need some additional conditions about free variables, I'd like to use what I defined above
@@ -9,4 +62,3 @@ lemma sub_comm (m n : ℕ) (t1 t2 t3 : Term)
   := sorry
 
 theorem unshiftSubstSwap {n : ℕ} (t1 t2 : Term) : (t1 [n+1 := t2.shift]).unshift = (t1.unshift [n := t2]) := sorry
-
